experiment/Experiment.Steel.Repr.M.fst
@@ -9,70 +9,35 @@ module L = FStar.List.Pure
 
 inline_for_extraction noextract
 let steel_of_repr
+      (#ek : SH.effect_kind)
       (#a : Type) (#pre : SE.pre_t) (#post : SE.post_t a) (#req : SE.req_t pre) (#ens : SE.ens_t pre a post)
       (tr : to_repr_t a pre post req ens)
-      (f : repr_steel_t SH.KSteel a tr.r_pre tr.r_post tr.r_req tr.r_ens)
-  : SH.unit_steel a pre post req ens
+      (f : repr_steel_t ek a tr.r_pre tr.r_post tr.r_req tr.r_ens)
+  : SH.steel a pre post req ens ek
   =
     (**) tr.r_pre_eq ();
     (**) FStar.Classical.forall_intro tr.r_post_eq;
     (**) FStar.Classical.forall_intro_2 reveal_equiv;
-    SH.unit_steel_subcomp_no_frame
+    SH.steel_subcomp_no_frame
       _ _ req ens
       (tr.r_pre_eq ()) (fun x -> tr.r_post_eq x)
       (SH.intro_subcomp_no_frame_pre _ _ _ _ _ _
         (fun h0      -> tr.r_req_eq h0)
         (fun h0 x h1 -> tr.r_ens_eq h0 x h1))
-      (SH.steel_u f)
-
-inline_for_extraction noextract
-let repr_steel_of_steel
-      (#a : Type) (#pre : SE.pre_t) (#post : SE.post_t a) (#req : SE.req_t pre) (#ens : SE.ens_t pre a post)
-      (tr : to_repr_t a pre post req ens)
-      ($f  : SH.unit_steel a pre post req ens)
-  : repr_steel_t SH.KSteel a tr.r_pre tr.r_post tr.r_req tr.r_ens
-  =
-    (**) tr.r_pre_eq ();
-    (**) FStar.Classical.forall_intro tr.r_post_eq;
-    (**) FStar.Classical.forall_intro_2 reveal_equiv;
-    SH.steel_f (SH.unit_steel_subcomp_no_frame
-      req ens _ _
-      () (fun _ -> ())
-      (SH.intro_subcomp_no_frame_pre _ _ _ _ _ _
-        (fun (h0 : hmem (vprop_of_list tr.r_pre)) ->
-           tr.r_req_eq h0)
-        (fun (h0 : hmem (vprop_of_list tr.r_pre)) x (h1 : hmem (vprop_of_list (tr.r_post x))) ->
-           tr.r_ens_eq h0 x h1))
-      f)
-
-inline_for_extraction noextract
-let steel_ghost_of_repr
-      #a #opened (#pre : SE.pre_t) (#post : SE.post_t a) (#req : SE.req_t pre) (#ens : SE.ens_t pre a post)
-      (tr : to_repr_t a pre post req ens)
       f
-  =
-    (**) tr.r_pre_eq ();
-    (**) FStar.Classical.forall_intro tr.r_post_eq;
-    (**) FStar.Classical.forall_intro_2 reveal_equiv;
-    SH.unit_steel_ghost_subcomp_no_frame #a #opened
-      _ _ req ens
-      (tr.r_pre_eq ()) (fun x -> tr.r_post_eq x)
-      (SH.intro_subcomp_no_frame_pre _ _ _ _ _ _
-        (fun h0      -> tr.r_req_eq h0)
-        (fun h0 x h1 -> tr.r_ens_eq h0 x h1))
-      (SH.ghost_u f)
 
 inline_for_extraction noextract
-let repr_steel_of_steel_ghost
-      #a #opened (#pre : SE.pre_t) (#post : SE.post_t a) (#req : SE.req_t pre) (#ens : SE.ens_t pre a post)
+let repr_of_steel
+      (#ek : SH.effect_kind)
+      (#a : Type) (#pre : SE.pre_t) (#post : SE.post_t a) (#req : SE.req_t pre) (#ens : SE.ens_t pre a post)
       (tr : to_repr_t a pre post req ens)
-      ($f  : SH.unit_steel_ghost a opened pre post req ens)
-  : repr_steel_t (SH.KGhost opened) a tr.r_pre tr.r_post tr.r_req tr.r_ens
+      ($f  : SH.steel a pre post req ens ek)
+  : repr_steel_t ek a tr.r_pre tr.r_post tr.r_req tr.r_ens
   =
     (**) tr.r_pre_eq ();
     (**) FStar.Classical.forall_intro tr.r_post_eq;
     (**) FStar.Classical.forall_intro_2 reveal_equiv;
-    SH.ghost_f #opened (SH.unit_steel_ghost_subcomp_no_frame
+    SH.steel_subcomp_no_frame
       req ens _ _
       () (fun _ -> ())
       (SH.intro_subcomp_no_frame_pre _ _ _ _ _ _
@@ -80,16 +45,17 @@ let repr_steel_of_steel_ghost
            tr.r_req_eq h0)
         (fun (h0 : hmem (vprop_of_list tr.r_pre)) x (h1 : hmem (vprop_of_list (tr.r_post x))) ->
            tr.r_ens_eq h0 x h1))
-      f)
+      f
 
 
 #push-options "--ifuel 0 --fuel 0"
 inline_for_extraction noextract
-let spec_r_of_find_ro
+let spec_r_of_find_ro__steel
       (#a : Type) (#pre : pre_t) (#post : post_t a) (#req : req_t pre) (#ens : ens_t pre a post)
       (sro : spec_find_ro a pre post req ens)
       (f : repr_steel_t SH.KSteel a pre post req ens)
-  = fun () ->
+  : spc_steel_t SH.KSteel sro.sro_spc
+  = SH.steel_f (fun () ->
       (**) let sl0    = gget_f sro.sro_spc.spc_pre in
       (**) let sl_fr0 = gget_f sro.sro_spc.spc_ro  in
       (**) intro_vpl_append sro.sro_spc.spc_pre sro.sro_spc.spc_ro;
@@ -103,20 +69,65 @@ let spec_r_of_find_ro
       (**) let sl1    = gget_f (sro.sro_spc.spc_post x) in
       (**) let sl_fr1 = gget_f sro.sro_spc.spc_ro       in
       (**) sro.sro_ens_eq sl0 sl_fr0 x sl1 sl_fr1;
-      Steel.Effect.Atomic.return x
+      Steel.Effect.Atomic.return x)
 
 inline_for_extraction noextract
-let spec_r_of_find_ro_ghost
+let spec_r_of_find_ro__atomic
       (#a : Type) (#pre : pre_t) (#post : post_t a) (#req : req_t pre) (#ens : ens_t pre a post)
       (sro : spec_find_ro a pre post req ens)
-      (#opened : Mem.inames) (f : repr_steel_t (SH.KGhost opened) a pre post req ens)
-  = fun () ->
+      (#opened : Mem.inames) (f : repr_steel_t (SH.KAtomic opened) a pre post req ens)
+  : spc_steel_t (SH.KAtomic opened) sro.sro_spc
+  = SH.atomic_f (fun () ->
       (**) let sl0    = gget_f sro.sro_spc.spc_pre in
       (**) let sl_fr0 = gget_f sro.sro_spc.spc_ro  in
       (**) intro_vpl_append sro.sro_spc.spc_pre sro.sro_spc.spc_ro;
       (**) change_vpl_perm sro.sro_pre_eq;
       (**) sro.sro_req_eq sl0 sl_fr0;
-      let (x : a) = SH.ghost_u f ()     in
+      let (x : a) = SH.atomic_u f ()    in
+      (**) let sl1'   = gget_f (post x) in
+      (**) change_vpl_perm (sro.sro_post_eq x);
+      (**) extract_vars_sym_l (sro.sro_post_eq x) sl1';
+      (**) elim_vpl_append (sro.sro_spc.spc_post x) sro.sro_spc.spc_ro;
+      (**) let sl1    = gget_f (sro.sro_spc.spc_post x) in
+      (**) let sl_fr1 = gget_f sro.sro_spc.spc_ro       in
+      (**) sro.sro_ens_eq sl0 sl_fr0 x sl1 sl_fr1;
+      Steel.Effect.Atomic.return x)
+
+inline_for_extraction noextract
+let spec_r_of_find_ro__ghostI
+      (#a : Type) (#pre : pre_t) (#post : post_t a) (#req : req_t pre) (#ens : ens_t pre a post)
+      (sro : spec_find_ro a pre post req ens)
+      (#opened : Mem.inames) (f : repr_steel_t (SH.KGhostI opened) a pre post req ens)
+  : spc_steel_t (SH.KGhostI opened) sro.sro_spc
+  = SH.ghostI_f (fun () ->
+      (**) let sl0    = gget_f sro.sro_spc.spc_pre in
+      (**) let sl_fr0 = gget_f sro.sro_spc.spc_ro  in
+      (**) intro_vpl_append sro.sro_spc.spc_pre sro.sro_spc.spc_ro;
+      (**) change_vpl_perm sro.sro_pre_eq;
+      (**) sro.sro_req_eq sl0 sl_fr0;
+      let (x : a) = SH.ghostI_u f ()    in
+      (**) let sl1'   = gget_f (post x) in
+      (**) change_vpl_perm (sro.sro_post_eq x);
+      (**) extract_vars_sym_l (sro.sro_post_eq x) sl1';
+      (**) elim_vpl_append (sro.sro_spc.spc_post x) sro.sro_spc.spc_ro;
+      (**) let sl1    = gget_f (sro.sro_spc.spc_post x) in
+      (**) let sl_fr1 = gget_f sro.sro_spc.spc_ro       in
+      (**) sro.sro_ens_eq sl0 sl_fr0 x sl1 sl_fr1;
+      Steel.Effect.Atomic.return x)
+
+inline_for_extraction noextract
+let spec_r_of_find_ro__ghost
+      (#a : Type) (#pre : pre_t) (#post : post_t a) (#req : req_t pre) (#ens : ens_t pre a post)
+      (sro : spec_find_ro a pre post req ens)
+      (#opened : Mem.inames) (f : repr_steel_t (SH.KGhost opened) a pre post req ens)
+  : spc_steel_t (SH.KGhost opened) sro.sro_spc
+  = SH.ghost_f (fun () ->
+      (**) let sl0    = gget_f sro.sro_spc.spc_pre in
+      (**) let sl_fr0 = gget_f sro.sro_spc.spc_ro  in
+      (**) intro_vpl_append sro.sro_spc.spc_pre sro.sro_spc.spc_ro;
+      (**) change_vpl_perm sro.sro_pre_eq;
+      (**) sro.sro_req_eq sl0 sl_fr0;
+      let (x : a) = SH.ghost_u f ()    in
       (**) let sl1'   = gget_f (post x) in
       (**) change_vpl_perm (sro.sro_post_eq x);
       (**) extract_vars_sym_l (sro.sro_post_eq x) sl1';
@@ -125,7 +136,20 @@ let spec_r_of_find_ro_ghost
       (**) let sl_fr1 = gget_f sro.sro_spc.spc_ro       in
       (**) sro.sro_ens_eq sl0 sl_fr0 x sl1 sl_fr1;
       noop ();
-      x
+      x)
+
 #pop-options
+
+inline_for_extraction noextract
+let spec_r_of_find_ro
+      (#a : Type) (#pre : pre_t) (#post : post_t a) (#req : req_t pre) (#ens : ens_t pre a post)
+      (sro : spec_find_ro a pre post req ens)
+      (#ek : SH.effect_kind) (f : repr_steel_t ek a pre post req ens)
+  : spc_steel_t ek sro.sro_spc
+  = match ek with
+  | SH.KSteel    -> spec_r_of_find_ro__steel  sro f
+  | SH.KAtomic o -> spec_r_of_find_ro__atomic sro #o f
+  | SH.KGhostI o -> spec_r_of_find_ro__ghostI sro #o f
+  | SH.KGhost  o -> spec_r_of_find_ro__ghost  sro #o f
 
 (**) private let __end_spec_r_of_find_ro = ()
