experiment/Experiment.Steel.Steel.fst
@@ -28,6 +28,47 @@ let focus_rmem_mkrmem (p q : vprop) (h : hmem p)
       with _ by T.(trefl ());
     Fext.extensionality_g _ _ (focus_rmem (mk_rmem p h) q) (mk_rmem q h)
 
+
+inline_for_extraction
+let steel_c #a #pre #post #req #ens (f : steel a pre post req ens KSteel)
+  : unit_steel a pre post req ens
+  = FSteel?.f f
+
+inline_for_extraction
+let atomic_c #opened #a #pre #post #req #ens (f : steel a pre post req ens (KAtomic opened))
+  : unit_steel_atomic a opened pre post req ens
+  = U.cast _ (FAtomic?.f f)
+
+inline_for_extraction
+let ghost_c #opened #a #pre #post #req #ens (f : steel a pre post req ens (KGhost opened))
+  : unit_steel_ghost a opened pre post req ens
+  = U.cast _ (FGhost?.f f)
+
+inline_for_extraction
+let ghostI_c #opened #a #pre #post #req #ens (f : steel a pre post req ens (KGhostI opened))
+  : unit_steel_ghostI a opened pre post req ens
+  = U.cast _ (FGhostI?.f f)
+
+
+(***** Subcomp *)
+
+#push-options "--ifuel 1 --fuel 1"
+inline_for_extraction noextract
+let steel_subcomp #ek a pre_f post_f req_f ens_f pre_g post_g req_g ens_g frame pr p1 p2 sc $f
+  = match f with
+  | FSteel f ->
+      FSteel (steel_subcomp__steel a pre_f post_f req_f ens_f pre_g post_g req_g ens_g frame pr p1 p2 sc f)
+  | FAtomic o f ->
+      FAtomic o (steel_subcomp__atomic Observable Observable a o
+                   pre_f post_f req_f ens_f pre_g post_g req_g ens_g frame pr p1 p2 () sc f)
+  | FGhostI o f ->
+      FGhostI o (steel_subcomp__atomic Unobservable Unobservable a o
+                   pre_f post_f req_f ens_f pre_g post_g req_g ens_g frame pr p1 p2 () sc f)
+  | FGhost o f ->
+      FGhost o (steel_subcomp__ghost a o
+                   pre_f post_f req_f ens_f pre_g post_g req_g ens_g frame pr p1 p2 sc f)
+#pop-options
+
 let intro_subcomp_no_frame_pre0
       (#a:Type)
       (#pre_f:pre_t) (#post_f:post_t a) (req_f:req_t pre_f) (ens_f:ens_t pre_f a post_f)
@@ -103,36 +144,20 @@ let subcomp_no_frame_lem
     equiv_forall_elim post_g (fun x -> post_f x `star` emp)
 
 inline_for_extraction noextract
-let unit_steel_subcomp_no_frame
-      (#a : Type)
+let steel_subcomp_no_frame
+      (#ek: effect_kind) (#a : Type)
       (#pre_f:pre_t) (#post_f:post_t a) (req_f:req_t pre_f) (ens_f:ens_t pre_f a post_f)
       (#pre_g:pre_t) (#post_g:post_t a) (req_g:req_t pre_g) (ens_g:ens_t pre_g a post_g)
       (eq_pre  : squash (equiv pre_g pre_f))
       (eq_post : (x : a) -> squash (equiv (post_g x) (post_f x)))
       (sb_pre : squash (subcomp_no_frame_pre req_f ens_f req_g ens_g eq_pre eq_post))
-      (f : unit_steel a pre_f post_f req_f ens_f)
-  : unit_steel a pre_g post_g req_g ens_g
+      (f : steel a pre_f post_f req_f ens_f ek)
+  : steel a pre_g post_g req_g ens_g ek
   =
     subcomp_no_frame_lem req_f ens_f req_g ens_g eq_pre eq_post;
     intro_subcomp_pre' req_f ens_f req_g ens_g #emp #True () ()
       (fun h0 -> ()) (fun h0 -> ()) (fun h0 x h1 -> ());
     steel_subcomp a
-      pre_f post_f req_f ens_f
-      pre_g post_g req_g ens_g
-      emp True () () ()
-      f
-
-inline_for_extraction noextract
-let unit_steel_ghost_subcomp_no_frame
-      #a #opened
-      #pre_f #post_f req_f ens_f
-      #pre_g #post_g req_g ens_g
-      eq_pre eq_post sb_pre f
-  =
-    subcomp_no_frame_lem req_f ens_f req_g ens_g eq_pre eq_post;
-    intro_subcomp_pre' req_f ens_f req_g ens_g #emp #True () ()
-      (fun h0 -> ()) (fun h0 -> ()) (fun h0 x h1 -> ());
-    steel_ghost_subcomp a opened
       pre_f post_f req_f ens_f
       pre_g post_g req_g ens_g
       emp True () () ()
