experiment/Experiment.Steel.Steel.fsti
@@ -31,6 +31,133 @@ val change_can_be_split_slprop
   : SteelGhost unit opened p (fun () -> q) (fun _ -> True) (fun h0 () h1 -> h1 q == h0 q)
 *)
 
+
+// ALT? Merge KAtomic & KGhostI
+noeq
+type effect_kind =
+  | KSteel
+  | KAtomic of Mem.inames
+  // Informative Ghost
+  | KGhostI of Mem.inames
+  | KGhost  of Mem.inames
+
+noeq inline_for_extraction
+type steel (a : Type) (pre : pre_t) (post : post_t a) (req : req_t pre) (ens : ens_t pre a post)
+  : effect_kind -> Type =
+  | FSteel  : (f : unit_steel a pre post req ens) ->
+               steel a pre post req ens KSteel
+  | FAtomic : (o : Mem.inames) -> (f : unit_steel_atomic a o pre post req ens) ->
+               steel a pre post req ens (KAtomic o)
+  | FGhostI : (o : Mem.inames) -> (f : unit_steel_ghostI a o pre post req ens) ->
+               steel a pre post req ens (KGhostI o)
+  | FGhost  : (o : Mem.inames) -> (f : unit_steel_ghost  a o pre post req ens) ->
+               steel a pre post req ens (KGhost o)
+
+
+unfold inline_for_extraction
+let steel_u #a #pre #post #req #ens (f : steel a pre post req ens KSteel)
+  : unit_steel a pre post req ens
+  = FSteel?.f f
+
+inline_for_extraction
+val steel_c (#a : Type) (#pre : pre_t) (#post : post_t a) (#req : req_t pre) (#ens : ens_t pre a post)
+            (f : steel a pre post req ens KSteel)
+  : unit_steel a pre post req ens
+
+unfold inline_for_extraction
+let steel_f #a #pre #post #req #ens (f : unit_steel a pre post req ens)
+  : steel a pre post req ens KSteel
+  = FSteel f
+
+unfold inline_for_extraction
+let steel_fe #a #pre #post #req #ens ($f : unit_steel a pre post req ens)
+  : steel a pre post req ens KSteel
+  = FSteel f
+
+
+unfold inline_for_extraction
+let atomic_u #opened #a #pre #post #req #ens (f : steel a pre post req ens (KAtomic opened))
+  : unit_steel_atomic a opened pre post req ens
+  = U.cast _ (FAtomic?.f f)
+
+inline_for_extraction
+val atomic_c (#opened : Mem.inames)
+             (#a : Type) (#pre : pre_t) (#post : post_t a) (#req : req_t pre) (#ens : ens_t pre a post)
+             (f : steel a pre post req ens (KAtomic opened))
+  : unit_steel_atomic a opened pre post req ens
+
+unfold inline_for_extraction
+let atomic_f #opened #a #pre #post #req #ens (f : unit_steel_atomic a opened pre post req ens)
+  : steel a pre post req ens (KAtomic opened)
+  = FAtomic opened f
+
+unfold inline_for_extraction
+let atomic_fe #opened #a #pre #post #req #ens ($f : unit_steel_atomic a opened pre post req ens)
+  : steel a pre post req ens (KAtomic opened)
+  = FAtomic opened f
+
+
+unfold inline_for_extraction
+let ghost_u #opened #a #pre #post #req #ens (f : steel a pre post req ens (KGhost opened))
+  : unit_steel_ghost a opened pre post req ens
+  = U.cast (unit_steel_ghost a opened pre post req ens) (FGhost?.f f)
+
+inline_for_extraction
+val ghost_c (#opened : Mem.inames)
+             (#a : Type) (#pre : pre_t) (#post : post_t a) (#req : req_t pre) (#ens : ens_t pre a post)
+             (f : steel a pre post req ens (KGhost opened))
+  : unit_steel_ghost a opened pre post req ens
+
+unfold inline_for_extraction
+let ghost_f #opened #a #pre #post #req #ens (f : unit_steel_ghost a opened pre post req ens)
+  : steel a pre post req ens (KGhost opened)
+  = FGhost opened f
+
+unfold inline_for_extraction
+let ghost_fe #opened #a #pre #post #req #ens ($f : unit_steel_ghost a opened pre post req ens)
+  : steel a pre post req ens (KGhost opened)
+  = FGhost opened f
+
+
+unfold inline_for_extraction
+let ghostI_u #opened #a #pre #post #req #ens (f : steel a pre post req ens (KGhostI opened))
+  : unit_steel_ghostI a opened pre post req ens
+  = U.cast (unit_steel_ghostI a opened pre post req ens) (FGhostI?.f f)
+
+inline_for_extraction
+val ghostI_c (#opened : Mem.inames)
+             (#a : Type) (#pre : pre_t) (#post : post_t a) (#req : req_t pre) (#ens : ens_t pre a post)
+             (f : steel a pre post req ens (KGhostI opened))
+  : unit_steel_ghostI a opened pre post req ens
+
+unfold inline_for_extraction
+let ghostI_f #opened #a #pre #post #req #ens (f : unit_steel_ghostI a opened pre post req ens)
+  : steel a pre post req ens (KGhostI opened)
+  = FGhostI opened f
+
+unfold inline_for_extraction
+let ghostI_fe #opened #a #pre #post #req #ens ($f : unit_steel_ghostI a opened pre post req ens)
+  : steel a pre post req ens (KGhostI opened)
+  = FGhostI opened f
+
+
+(***** Subcomp *)
+
+inline_for_extraction noextract
+val steel_subcomp
+      (#ek : effect_kind) (a:Type)
+      (pre_f:pre_t)       (post_f:post_t a)
+      (req_f:req_t pre_f) (ens_f:ens_t pre_f a post_f)
+      (pre_g:pre_t)       (post_g:post_t a)
+      (req_g:req_t pre_g) (ens_g:ens_t pre_g a post_g)
+      (frame:vprop)
+      (pr : prop)
+      (p1 : squash (can_be_split_dep pr pre_g (pre_f `star` frame)))
+      (p2 : squash (equiv_forall post_g (fun x -> post_f x `star` frame)))
+      (sc : squash (subcomp_pre' req_f ens_f req_g ens_g p1 p2))
+      ($f : steel a pre_f post_f req_f ens_f ek)
+  : steel a pre_g post_g req_g ens_g ek
+
 let subcomp_no_frame_pre
       (#a:Type)
       (#pre_f:pre_t) (#post_f:post_t a) (req_f:req_t pre_f) (ens_f:ens_t pre_f a post_f)
@@ -68,84 +195,12 @@ val intro_subcomp_no_frame_pre
   : squash (subcomp_no_frame_pre req_f ens_f req_g ens_g eq_pre eq_post)
 
 inline_for_extraction noextract
-val unit_steel_subcomp_no_frame
-      (#a : Type)
+val steel_subcomp_no_frame
+      (#ek : effect_kind) (#a : Type)
       (#pre_f:pre_t) (#post_f:post_t a) (req_f:req_t pre_f) (ens_f:ens_t pre_f a post_f)
       (#pre_g:pre_t) (#post_g:post_t a) (req_g:req_t pre_g) (ens_g:ens_t pre_g a post_g)
       (eq_pre  : squash (equiv pre_g pre_f))
       (eq_post : (x : a) -> squash (equiv (post_g x) (post_f x)))
       (sb_pre : squash (subcomp_no_frame_pre req_f ens_f req_g ens_g eq_pre eq_post))
-      ($f : unit_steel a pre_f post_f req_f ens_f)
-  : unit_steel a pre_g post_g req_g ens_g
-
-inline_for_extraction noextract
-val unit_steel_ghost_subcomp_no_frame
-      (#a : Type) (#opened : Mem.inames)
-      (#pre_f:pre_t) (#post_f:post_t a) (req_f:req_t pre_f) (ens_f:ens_t pre_f a post_f)
-      (#pre_g:pre_t) (#post_g:post_t a) (req_g:req_t pre_g) (ens_g:ens_t pre_g a post_g)
-      (eq_pre  : squash (equiv pre_g pre_f))
-      (eq_post : (x : a) -> squash (equiv (post_g x) (post_f x)))
-      (sb_pre : squash (subcomp_no_frame_pre req_f ens_f req_g ens_g eq_pre eq_post))
-      ($f : unit_steel_ghost a opened pre_f post_f req_f ens_f)
-  : unit_steel_ghost a opened pre_g post_g req_g ens_g
-
-
-noeq
-type effect_kind =
-  | KSteel
-  | KAtomic of Mem.inames
-  // Informative Ghost
-  | KGhostI of Mem.inames
-  | KGhost  of Mem.inames
-
-noeq inline_for_extraction
-type steel (a : Type) (pre : pre_t) (post : post_t a) (req : req_t pre) (ens : ens_t pre a post)
-  : effect_kind -> Type =
-  | FSteel  : (f : unit_steel a pre post req ens) ->
-               steel a pre post req ens KSteel
-  | FAtomic : (o : Mem.inames) -> (f : unit_steel_atomic a o pre post req ens) ->
-               steel a pre post req ens (KAtomic o)
-  | FGhostI : (o : Mem.inames) -> (f : unit_steel_ghostI a o pre post req ens) ->
-               steel a pre post req ens (KGhostI o)
-  | FGhost  : (o : Mem.inames) -> (f : unit_steel_ghost  a o pre post req ens) ->
-               steel a pre post req ens (KGhost o)
-
-unfold inline_for_extraction
-let steel_u #a #pre #post #req #ens (f : steel a pre post req ens KSteel)
-  : unit_steel a pre post req ens
-  = FSteel?.f f
-
-unfold inline_for_extraction
-let steel_f #a #pre #post #req #ens (f : unit_steel a pre post req ens)
-  : steel a pre post req ens KSteel
-  = FSteel f
-
-unfold inline_for_extraction
-let atomic_u #opened #a #pre #post #req #ens (f : steel a pre post req ens (KAtomic opened))
-  : unit_steel_atomic a opened pre post req ens
-  = U.cast _ (FAtomic?.f f)
-
-unfold inline_for_extraction
-let atomic_f #opened #a #pre #post #req #ens (f : unit_steel_atomic a opened pre post req ens)
-  : steel a pre post req ens (KAtomic opened)
-  = FAtomic opened f
-
-unfold inline_for_extraction
-let ghost_u #opened #a #pre #post #req #ens (f : steel a pre post req ens (KGhost opened))
-  : unit_steel_ghost a opened pre post req ens
-  = U.cast (unit_steel_ghost a opened pre post req ens) (FGhost?.f f)
-
-unfold inline_for_extraction
-let ghost_f #opened #a #pre #post #req #ens (f : unit_steel_ghost a opened pre post req ens)
-  : steel a pre post req ens (KGhost opened)
-  = FGhost opened f
-
-unfold inline_for_extraction
-let ghostI_u #opened #a #pre #post #req #ens (f : steel a pre post req ens (KGhostI opened))
-  : unit_steel_ghostI a opened pre post req ens
-  = U.cast (unit_steel_ghostI a opened pre post req ens) (FGhostI?.f f)
-
-unfold inline_for_extraction
-let ghostI_f #opened #a #pre #post #req #ens (f : unit_steel_ghostI a opened pre post req ens)
-  : steel a pre post req ens (KGhostI opened)
-  = FGhostI opened f
+      ($f : steel a pre_f post_f req_f ens_f ek)
+  : steel a pre_g post_g req_g ens_g ek
